LR for normalization STLC (WIP)

theories/normalization.v
@@ -21,7 +21,7 @@ Fixpoint substitute γ e :=
   end.
 
 Definition normalize_to_v e v :=
-  is_val v -> e ~>* v.
+  is_val v /\ e ~>* v.
 
 Definition normalize e :=
   exists v, normalize_to_v e v.
@@ -42,8 +42,8 @@ Definition sem_subst γ Γ :=
                       | Some t => t
                     end)
                   (substitute γ (expr_var x)))
-    (domain γ).
-  (* dom Γ = domain γ. *)
+    (domain γ) /\
+  (map_to_list Γ).*1 = domain γ.
 Notation " γ ⊨ Γ" := (sem_subst γ Γ) (at level 99).
 Lemma sn_safe : forall τ e, sn τ e -> ⇓ e.
 Proof.
@@ -55,19 +55,54 @@ Lemma substitution_lemma Γ γ τ e :
   Γ ⊢ e ∈ τ ->
   γ ⊨ Γ ->
   (typing_judgment ∅ (substitute γ e) τ).
+Proof.
 Admitted.
+
+Lemma substitution_preserves_typing :
+  ∀ (Γ : context) (x: string) v τx e τ,
+  is_val v ->
+  (typing_judgment (<[x := τx]> Γ) e τ) ->
+  (typing_judgment ∅ v τx) ->
+  (typing_judgment Γ (subst_term x v e) τ).
+Proof.
+Admitted.
+
+
+Lemma preservation :
+  forall e e' τ, (∅ ⊢ e ∈ τ) ->
+            e ~> e' ->
+            (∅ ⊢ e' ∈ τ).
+Proof.
+  intros * Ht ?.
+  generalize dependent e'.
+  remember empty as Γ.
+  induction Ht;
+       intros * HE; subst;
+       try solve [inversion HE; subst; auto].
+  inversion_clear HE; subst;eauto.
+  eapply substitution_preserves_typing; eauto.
+    admit.
+Admitted.
+
 
 Lemma sn_backward τ e e':
  (∅ ⊢ e ∈ τ) ->
  e ~> e' ->
  (sn τ e' -> sn τ e).
+Proof.
 Admitted.
 
 Lemma sn_backward_star τ e e':
  (∅ ⊢ e ∈ τ) ->
  e ~>* e' ->
  (sn τ e' -> sn τ e).
-Admitted.
+Proof.
+  intros.
+  induction H0 using star_ind; auto.
+  eapply sn_backward; eauto.
+  apply IHstar;auto.
+  eapply preservation;eauto.
+Qed.
 
 Lemma sn_forward τ e e':
  (∅ ⊢ e ∈ τ) ->
@@ -79,7 +114,13 @@ Lemma sn_forward_star τ e e':
  (∅ ⊢ e ∈ τ) ->
  e ~>* e' ->
  (sn τ e -> sn τ e').
-Admitted.
+Proof.
+  intros.
+  induction H0 using star_ind; auto.
+  apply IHstar;auto.
+  eapply preservation;eauto.
+  eapply sn_forward; eauto.
+Qed.
 
 Lemma sn_well_typed τ e: sn τ e -> (∅ ⊢ e ∈ τ).
 Proof.
@@ -93,6 +134,11 @@ Lemma substitute_false γ :
 (substitute γ <{ false }> ) = <{false}>.
 Admitted.
 
+Lemma substitute_abs γ x e  :
+(substitute γ <{ λ x, e }>) =
+  expr_abs x (substitute γ <{ e }>).
+Admitted.
+
 Lemma substitute_app γ e e' :
 (substitute γ <{ e e' }>) =
   expr_app (substitute γ <{ e }>) (substitute γ <{ e' }>).
@@ -103,70 +149,176 @@ Lemma substitute_if γ e e1 e2 :
   expr_if (substitute γ <{ e }>) (substitute γ <{ e1 }>) (substitute γ <{ e2 }>).
 Admitted.
 
-Lemma fundamental : forall Γ γ τ e,
-  (Γ ⊢ e ∈ τ) ->
+Lemma substitute_neq_commute γ x1 x2 e e1 e2:
+  (x1 ≠ x2)%string ->
+  substitute γ <{ [x1 / e1] ([x2 / e2] e) }>
+    =
+  substitute γ <{ [x2 / e2] ([x1 / e1] e) }>.
+Admitted.
+
+Lemma substitute_eq_update γ x e e1 e2:
+  substitute γ <{ [x / e1] ([x / e2] e) }>
+    =
+  substitute γ <{ [x / e1] e }>.
+Admitted.
+
+Lemma subst_term_substitute:
+  ∀ γ (x : string) (e : expr) (v : val),
+  subst_term x (of_val v) (substitute γ e)
+  = substitute ((x, v) :: γ) e.
+Proof.
+  intros; cbn.
+  generalize dependent x.
+  generalize dependent v.
+  generalize dependent e.
+  induction γ;auto;intros.
+  destruct a;cbn.
+  destruct (s =? x)%string eqn:Heq.
+  - apply String.eqb_eq in Heq; subst.
+    rewrite substitute_eq_update.
+    rewrite <- IHγ.
+    admit.
+  -apply String.eqb_neq in Heq; subst.
+    rewrite substitute_neq_commute; auto.
+Admitted.
+
+Lemma sem_subst_empty Γ :
+ [] ⊨ Γ -> Γ = ∅.
+Proof.
+  intros.
+  inversion H.
+  simpl in*.
+  apply fmap_nil_inv in H1.
+  by apply map_to_list_empty_iff.
+Qed.
+
+Lemma sem_subst_cons: forall Γ γ x v τ,
   γ ⊨ Γ ->
+  sn τ (of_val v) ->
+  (x, v) :: γ ⊨ <[x:=τ]> Γ.
+Proof.
+  induction γ;intros.
+  - apply sem_subst_empty in H ; subst.
+    unfold sem_subst ; cbn.
+    split.
+    + apply Forall_singleton.
+    replace (<[x:=τ]> ∅ !! x) with (Some τ) by
+                                   (symmetry; apply lookup_insert).
+    rewrite String.eqb_refl; auto.
+    + replace (<[x:=τ]> ∅) with (singletonM x τ : gmap string ty) by auto.
+    setoid_rewrite map_to_list_singleton; auto.
+  - destruct a as [x' v'].
+    admit.
+    (* inversion_clear H. *)
+Admitted.
+
+Lemma some_in_context :
+  forall l Γ x τ,
+  Γ !! x = Some τ ->
+  (map_to_list Γ).*1 = l ->
+  x ∈ l.
+Proof.
+  induction l; intros.
+  - apply fmap_nil_inv in H0.
+    apply map_to_list_empty_iff in H0;subst.
+    discriminate H.
+  - assert ( Hinv: exists Γ' τ', Γ = <[ a := τ']> Γ' ).
+    admit.
+    destruct Hinv as ( Γ' & τ' & -> ).
+    assert ( (map_to_list Γ').*1 = l). admit.
+    destruct (x =? a)%string eqn:Heq.
+    + apply String.eqb_eq in Heq; subst.
+      apply elem_of_list_here.
+    +  apply String.eqb_neq in Heq; subst.
+      apply elem_of_list_further.
+      eapply (IHl Γ' _ τ); auto.
+      setoid_rewrite lookup_insert_ne in H; auto.
+Admitted.
+
+Lemma fundamental : forall Γ γ τ e,
+  γ ⊨ Γ ->
+  (Γ ⊢ e ∈ τ) ->
   sn τ (substitute γ e).
 Proof.
-  induction 1 ; simpl in *; intros.
+  intros; generalize dependent γ.
+  induction H0; intros ; simpl in *.
   - (* true *)
     split; rewrite substitute_true; auto.
-    eexists; intro; eapply star_refl.
+    eexists;split;try eapply star_refl;eauto.
   - (* false *)
     split; rewrite substitute_false; auto.
-    eexists; intro; eapply star_refl.
-  - (* var *) admit.
+    eexists;split;try eapply star_refl;eauto.
+  - (* var *)
+    destruct H0 as [ ? Hdom ].
+    assert (Hx: x ∈ (domain γ)) by (eapply some_in_context; eauto).
+    eapply Forall_forall in H0;eauto.
+    by rewrite H in H0.
+
   - (* lam *)
     split.
     apply substitution_lemma with (Γ := Γ);auto.
-    split. admit.
-    intros.
+    rewrite substitute_abs.
+    split.
+    eexists;split;try eapply star_refl;eauto.
+    intros e' sn_e'.
+    pose proof sn_e' as Hsn_e'.
+    apply sn_safe in sn_e'; destruct sn_e' as (v & v_val & step_e').
+    apply sn_backward_star with (e' := expr_app (expr_abs x (substitute γ e)) v);auto.
     admit.
+    apply mstep_app_arg; auto.
+    apply sn_backward_star with (e' := subst_term x v (substitute γ e));auto.
+    admit.
+    apply star_one; auto.
+    apply is_val_inversion in v_val ; destruct v_val; subst.
+    rewrite subst_term_substitute.
+    apply IHtyping_judgment.
+    apply sem_subst_cons;auto.
+    eapply sn_forward_star in Hsn_e';eauto; apply sn_well_typed;assumption.
+
   - (* app *)
-    pose proof H1 as H2.
-    apply IHtyping_judgment1 in H1
+    pose proof H as H'.
+    apply IHtyping_judgment1 in H
     ; clear IHtyping_judgment1
-    ; destruct H1 as (IH1_type & IH1_norm & IH1_sn).
-    apply IHtyping_judgment2 in H2; clear IHtyping_judgment2.
+    ; destruct H as (IH1_type & IH1_norm & IH1_sn).
+    apply IHtyping_judgment2 in H'; clear IHtyping_judgment2.
     rewrite substitute_app.
     by apply IH1_sn.
+
   - (* if *)
-    pose proof H2 as H3;
-    pose proof H2 as H4.
-    apply IHtyping_judgment1 in H2
+    pose proof H as H1;
+    pose proof H as H2.
+    apply IHtyping_judgment1 in H
     ; clear IHtyping_judgment1
-    ; destruct H2 as [H_bool H_norm].
-    apply IHtyping_judgment2 in H3
+    ; destruct H as [H_bool H_norm].
+    apply IHtyping_judgment2 in H1
     ; clear IHtyping_judgment2.
-    apply IHtyping_judgment3 in H4
+    apply IHtyping_judgment3 in H2
     ; clear IHtyping_judgment3.
 
     destruct H_norm as [v H_norm].
     assert (Hv : (substitute γ e) ~>* <{ true }>
-                 \/ (substitute γ e) ~>* <{ false }> ).
+
     { admit. }
     destruct Hv.
     + (* true *)
       apply sn_backward_star
         with (e' := expr_if expr_true (substitute γ e1) (substitute γ e2)).
       rewrite substitute_if.
-      apply T_If; auto;
-      apply sn_well_typed;auto.
+      apply T_If; auto; apply sn_well_typed;auto.
       rewrite substitute_if.
-      admit.
+      apply mstep_if;auto.
       apply sn_backward_star with (e' := (substitute γ e1));auto.
-      admit.
+      apply T_If;auto; apply sn_well_typed;auto.
       apply star_one; auto.
     + (* false *)
       apply sn_backward_star
         with (e' := expr_if expr_false (substitute γ e1) (substitute γ e2)).
       rewrite substitute_if.
-      apply T_If; auto;
-      apply sn_well_typed;auto.
+      apply T_If; auto; apply sn_well_typed;auto.
       rewrite substitute_if.
-      admit.
+      apply mstep_if;auto.
       apply sn_backward_star with (e' := (substitute γ e2));auto.
-      admit.
+      apply T_If;auto; apply sn_well_typed;auto.
       apply star_one; auto.
 Admitted.
 
